Lista la biyección y la acción sobre el entorno.

src/Gen_Ext_Sep_test.thy
@@ -1,19 +1,290 @@
 theory Gen_Ext_Sep_test imports Forces_locale begin
 
 definition 
-  perm_sep_forces :: "i\<Rightarrow>i" where
-  "perm_sep_forces(n) == {\<langle>0, 4\<rangle>, \<langle>1, 3\<rangle>, \<langle>2, 7\<rangle>, \<langle>3, 0\<rangle>, \<langle>4, 1\<rangle>, \<langle>5, 2\<rangle>, \<langle>6, 5\<rangle>, \<langle>7, 6\<rangle>}"
+  f :: "i\<Rightarrow>i" where
+  "f(n) == {\<langle>0, 3\<rangle>, \<langle>1, 4\<rangle>, \<langle>2, 5\<rangle>, \<langle>3, 1\<rangle>, \<langle>4, 0\<rangle>, \<langle>5, 6\<rangle>, \<langle>6#+n, 2\<rangle>}"
 
-lemma perm_sep_bij: "perm_sep_forces(n) \<in> bij(n,n)" 
-  sorry
+lemma f_range : "range(f(n)) = 7"
+  by(unfold f_def,auto)
     
-lemma conv_perm_sep_bij: "converse(perm_sep_forces(n)) \<in> bij(n,n)" 
-  by (rule perm_sep_bij [THEN bij_converse_bij])
+definition 
+  fInv :: "i\<Rightarrow>i" where
+  "fInv(n) == {\<langle>3,0\<rangle>, \<langle>4,1\<rangle>, \<langle>5,2\<rangle>, \<langle>1,3\<rangle>, \<langle>0,4\<rangle>, \<langle>6,5\<rangle>, \<langle>2,6#+n\<rangle>}"
 
-lemma perm_sep_env: 
-  "perm_list(perm_sep_forces(length(env)#+7),[p,q,r,s,t,u]@env@[w]) = [t,s,w,p,q,r,u]@env"
-  sorry
+lemma f_ftc : "n \<in> nat \<Longrightarrow> f(n) \<in> (6 \<union> {6#+n}) -||> 7"
+  by (simp add : f_def,(rule consI,auto)+,rule emptyI)
+  
+lemma fInv_ftc : "n \<in> nat \<Longrightarrow> fInv(n) \<in> 7 -||> (6 \<union> {6#+n})"
+  by (simp add : fInv_def,(rule consI,auto)+,rule emptyI)
+
     
+lemma dom_f : "domain(f(n)) = 6 \<union> {6#+n}"
+  by(unfold f_def,auto)
+
+lemma dom_fInv : "domain(fInv(n)) = 7"     
+  by(unfold fInv_def,auto)
+    
+lemma f_tc: "n \<in> nat \<Longrightarrow> f(n) \<in> (6 \<union> {6#+n}) -> 7"
+  by(subst dom_f[symmetric],rule FiniteFun_is_fun,erule f_ftc)  
+
+lemma fInv_tc: "n \<in> nat \<Longrightarrow> fInv(n) \<in> 7 \<rightarrow> (6 \<union> {6#+n})"
+  by(subst dom_fInv[symmetric],rule FiniteFun_is_fun,erule fInv_ftc)  
+     
+lemma conv_f_eq : "n \<in> nat \<Longrightarrow> fInv(n) = converse(f(n))"
+  by(unfold fInv_def f_def,auto)
+
+lemma conv_fInv_eq : "n \<in> nat \<Longrightarrow> converse(fInv(n)) = f(n)"
+  by(unfold fInv_def f_def,auto)
+    
+lemma ble2 :  "i \<in> nat \<Longrightarrow> succ(j) \<in> i#+1 \<Longrightarrow> j \<in> i"
+  by(case_tac "j \<in> nat",auto simp add:nat_succD)
+
+lemma ble1 :  "j \<in> nat \<Longrightarrow> j \<noteq> 0 \<Longrightarrow> i \<in> nat \<Longrightarrow> j \<in> i#+1 \<Longrightarrow> pred(j) \<in> i"
+  by(rule natE[of "i"],simp+,blast,auto simp add : nat_succD succ_pred_eq)
+    
+definition 
+  gInv :: "i \<Rightarrow> i" where
+  "gInv(n) == \<lambda> j \<in> (7#+n)-7 . pred(j)"
+
+definition 
+  g :: "i \<Rightarrow> i" where
+  "g(n) == \<lambda> j \<in> (6#+n)-6 . succ(j)"
+
+    
+lemma g_tc : " g(n) \<in> ((6#+n)-6) \<rightarrow> (7#+n)-7"
+  apply(unfold g_def,rule lam_type)
+  apply(subgoal_tac "succ(j)< 7#+n" "j\<notin>6", rule DiffI,erule ltD)
+  apply(rule notI,simp add:ble2,rule notI,frule DiffD2,simp)
+  apply(frule DiffD1,subst add_succ,rule succ_leI,erule ltI,simp)
+done
+
+lemma gInv_tc : " gInv(n) \<in>  (7#+n)-7 \<rightarrow> ((6#+n)-6)"
+  apply(unfold gInv_def,rule lam_type)
+  apply(subgoal_tac "j \<notin> 7" "j \<noteq> 0" "j \<in> nat" "7#+ n =(6#+n)#+1",rule DiffI,rule ble1,simp+) 
+  apply(rule notI,subgoal_tac "j\<in>7",simp,frule ltI[of _ "6"],simp,subst succ_pred_eq[symmetric],simp+,rule nat_succI,simp+)
+  apply(rule in_n_in_nat,auto)
+done
+  
+lemma compUnEq : "B \<subseteq> A \<Longrightarrow> (A - B) \<union> B = A"
+  by(auto)
+
+lemma ble3 : "n \<in> nat \<Longrightarrow> 7#+n = ((6#+n) - 6) \<union> (6 \<union> {6#+n})"
+  apply (subgoal_tac "6 \<subseteq> 6#+n", subst Un_assoc[symmetric],subst compUnEq,simp,force)  
+  apply(rule le_imp_subset, rule add_le_self,simp)
+done
+    
+lemma ble4 : "n \<in> nat \<Longrightarrow> 7#+n = ((7#+n) - 7) \<union> 7"
+  by(subgoal_tac "7 \<subseteq> 7#+n",simp add:compUnEq,rule le_imp_subset, rule add_le_self,simp)
+    
+lemma disjI : "(\<forall> x \<in> A . x \<notin> B) \<Longrightarrow> (\<forall> x \<in> B . x \<notin> A) \<Longrightarrow> A \<inter> B \<subseteq> 0"
+  by(clarsimp)
+
+lemma ble5 : "(A - B) \<inter> (B \<union> {A}) = 0"
+  by(rule equalityI,simp_all, rule disjI,auto,erule mem_irrefl,erule mem_irrefl)
+
+lemma disjunctE : "A \<inter> B = 0 \<Longrightarrow> (\<forall> x \<in> A . x \<notin> B) \<and> (\<forall> x \<in> B . x \<notin> A)"
+  by(auto)
+    
+lemma ble6 : "A \<inter> B = 0 \<Longrightarrow> a \<in> A \<Longrightarrow> a \<notin> B" 
+  by(auto simp add: disjunctE ble5)
+
+lemma ble7 : "A \<inter> B = 0 \<Longrightarrow> a \<in> B \<Longrightarrow> a \<notin> A" 
+  by(rule ble6,subst Int_commute,simp+)
+    
+definition fUg :: "i \<Rightarrow> i" where
+  "fUg(n) = g(n) \<union> f(n)"
+
+definition fUgInv :: "i \<Rightarrow> i" where
+  "fUgInv(n) = gInv(n) \<union> fInv(n)"
+
+lemma fUg_tc : "n \<in> nat \<Longrightarrow> fUg(n) \<in> (7#+n) -> 7#+n"
+  apply(subst (1) ble3,assumption+)
+  apply(subst ble4,assumption+,unfold fUg_def)
+  apply(rule fun_disjoint_Un,rule g_tc,erule f_tc,rule ble5)
+done
+
+  
+lemma apply_fun: "fa \<in> Pi(A,B) ==> <a,b>: fa \<Longrightarrow> fa`a = b"
+  by(auto simp add: apply_iff)
+    
+lemma congIn : "a \<in> A \<Longrightarrow> A = B \<Longrightarrow> a\<in> B"
+  by auto
+
+lemma notSuccIn : "x \<in> nat \<Longrightarrow> y \<in> nat \<Longrightarrow> x \<notin> y \<Longrightarrow> succ(x) \<notin> succ(y)"
+  by(auto,drule ltI[of _ "y"],simp,subgoal_tac "x\<in>y",simp,rule ltD,rule lt_trans[of _ "succ(x)"],simp+)
+    
+lemma g_inj : "n \<in> nat \<Longrightarrow> g(n) \<in> inj((6#+n)-6,(7#+n)-7)"
+  apply(rule_tac d="\<lambda> x . gInv(n)`x" in f_imp_injective,rule g_tc)
+  apply(rule ballI)
+  apply(unfold gInv_def,subst beta,rule apply_type,rule g_tc,assumption)
+  apply(unfold g_def,subst beta,assumption)
+  apply(simp add: nat_succI)
+done
+
+
+lemma ble8 : "n \<in> nat \<Longrightarrow> y \<in> 7 #+ n - 7 \<Longrightarrow> Arith.pred(y) \<in> 6 #+ n - 6"
+  apply(subgoal_tac "y \<noteq>0",rule DiffI,rule ble1,rule in_n_in_nat[of "7#+n"],simp+)
+  prefer 2   apply(rule notI,simp,subgoal_tac "0\<in>7",simp,rule zero_in,simp)
+  apply(rule notI,subgoal_tac "succ(pred(y)) \<in> 7",subst (asm) succ_pred_eq)
+  apply(rule in_n_in_nat[of "7#+n"],simp+,rule nat_succI,simp+)
+done
+    
+lemma g_surj : "n \<in> nat\<Longrightarrow> g(n) \<in> surj(6#+n-6,7#+n-7)"
+  apply(rule_tac d="\<lambda> x . gInv(n)`x" in f_imp_surjective,rule g_tc)
+  apply(unfold gInv_def,subst beta,simp,rule ble8,simp+)
+  apply(unfold g_def,subst beta,rule ble8,simp+)
+  apply(subgoal_tac "y\<noteq>0",rule succ_pred_eq,rule in_n_in_nat[of "7#+n"],simp+)
+  apply(rule notI,simp,subgoal_tac "0\<in>7",simp,rule zero_in,simp)
+done
+
+lemma g_bij : "n \<in> nat\<Longrightarrow> g(n) \<in> bij(6#+n-6,7#+n-7)"
+  by(unfold bij_def,rule IntI,rule g_inj,simp, rule g_surj,simp)
+    
+lemma g_range : "n \<in> nat \<Longrightarrow> range(g(n)) = (7#+n)-7"
+  by(rule surj_range,erule g_surj)
+
+lemma conv_g_ap : "n \<in> nat \<Longrightarrow> i \<in> 7#+n -7 \<Longrightarrow> converse(g(n))`i = gInv(n)`i"
+  apply(rule left_inverse_eq,erule g_inj)
+   apply(unfold gInv_def,subst beta,assumption)
+  apply(unfold g_def,subst beta,rule ble8,simp+)  
+  apply(subgoal_tac "i\<noteq>0",rule succ_pred_eq,rule in_n_in_nat[of "7#+n"],simp+)
+  apply(rule notI,simp,subgoal_tac "0\<in>7",simp,rule zero_in,simp,subst beta,simp,rule ble8,simp+)
+done
+
+lemma conv_g_eq : "n \<in> nat \<Longrightarrow> converse(g(n)) = gInv(n)"
+  apply(rule fun_extension,rule inj_converse_fun, erule g_inj)
+   apply(subst g_range,simp,rule gInv_tc)
+  apply(rule conv_g_ap,simp,subst (asm) g_range,simp+)
+done
+  
+lemma fUg_inj: "n \<in> nat \<Longrightarrow> fUg(n) \<in> inj(7#+n,7#+n)"   
+  apply(rule_tac d="\<lambda> x . fUgInv(n)`x" in f_imp_injective, erule fUg_tc)
+  apply(clarify,drule_tac a="x" in congIn,erule ble3,rule_tac c="x" in UnE,assumption)
+   apply(unfold fUg_def fUgInv_def)
+   apply(subst fun_disjoint_apply1[of "x"],subst dom_f)
+    prefer 2 apply(subst fun_disjoint_apply1)
+    prefer 2 apply(unfold g_def,subst beta,simp,unfold gInv_def,subst beta)
+      prefer 4 apply(rule ble6, rule ble5,simp)
+     prefer 2 apply(rule pred_succ_eq)
+    prefer 3 
+       apply(subst fun_disjoint_apply2[of "x"],subst domain_lam,rule ble7,rule ble5,simp)
+    apply(subst fun_disjoint_apply2,subst domain_lam)
+     apply(rule notI,drule DiffD2,rule notE,assumption,rule apply_type,rule f_tc,simp+)
+    apply(subst conv_f_eq,simp,rule left_inverse_lemma,erule f_tc)
+  apply(subst conv_f_eq[symmetric],simp,erule fInv_tc,simp,rule DiffI,drule DiffD1)
+    apply(simp add: nat_succI,rule notSuccIn,simp,rule in_n_in_nat[of "6#+n"],simp+)
+    apply(subst dom_fInv,rule notSuccIn,rule in_n_in_nat[of "6#+n"],simp+)
+  done
+
+    
+lemma fUg_range : "n \<in> nat \<Longrightarrow> range(fUg(n)) = 7#+n"
+  apply(unfold fUg_def,subst range_Un_eq,subst ble4,simp,subst g_range,simp)
+  apply(subst f_range,simp)
+done
+lemma fUg_surj: "n \<in> nat \<Longrightarrow> fUg(n) \<in> surj(7#+n,7#+n)" 
+  by(subst (2) fUg_range[symmetric],simp,rule fun_is_surj,erule fUg_tc)
+  
+lemma fUg_bij: "n \<in> nat \<Longrightarrow> fUg(n) \<in> bij(7#+n,7#+n)" 
+  by(unfold bij_def,rule IntI,erule fUg_inj,erule fUg_surj)
+    
+lemma fUg_conv_bij: "n \<in> nat \<Longrightarrow> converse(fUg(n)) \<in> bij(7#+n,7#+n)" 
+  by (erule fUg_bij [THEN bij_converse_bij])
+
+lemma conv_fUg_eq: "n \<in> nat \<Longrightarrow> converse(fUg(n)) = fUgInv(n)" 
+  apply(unfold fUg_def fUgInv_def,subst converse_Un)
+  apply(subst conv_f_eq,simp,subst conv_g_eq,simp+) 
+done
+
+lemma ble0 : "f1 \<in> bij(a,b) \<Longrightarrow> g1 = converse(f1) \<Longrightarrow> converse(g1) = f1"
+  apply(subgoal_tac "g1 \<in> bij(b,a)",rule fun_extension)
+  apply(rule bij_is_fun,rule bij_converse_bij,simp,rule bij_is_fun,simp)
+   apply(rule left_inverse_eq,rule bij_is_inj,simp,simp,rule left_inverse_bij,simp+)
+   apply(rule apply_type,rule bij_is_fun,simp+)
+  done
+    
+lemma conv_fUgInv_eq: "n \<in> nat \<Longrightarrow> fUg(n) = converse(fUgInv(n))" 
+  apply(subst conv_fUg_eq[symmetric],simp)
+  apply(unfold fUg_def,subst converse_Un,subst converse_Un)
+  apply(subst conv_f_eq[symmetric],simp,subst conv_g_eq,simp+) 
+  apply(subst ble0[of "g(n)"],rule g_bij,simp,subst conv_g_eq,simp+) 
+  apply(subst conv_fInv_eq,simp+) 
+done
+
+  
+lemma fUgInv_bij : "n \<in> nat \<Longrightarrow> fUgInv(n) \<in>  bij(7#+n,7#+n)"
+  by(subst conv_fUg_eq[symmetric],simp,erule fUg_conv_bij)
+  
+lemma env_len : "{p,q,r,s,t,u,w} \<subseteq> M \<Longrightarrow> env \<in> list(M) \<Longrightarrow> length([p, q, r, s, t, u] @ env @ [w]) = 7#+length(env)"
+  by(simp)
+lemma env_len2 : "{p,q,r,s,t,u,w} \<subseteq> M \<Longrightarrow> env \<in> list(M) \<Longrightarrow> length([t,s,w,p,q,r,u] @ env) = 7#+length(env)"
+  by(simp)
+    
+lemma in7 : "i \<in> 7 \<Longrightarrow> i = 0 \<or> i = 1 \<or> i = 2 \<or> i = 3 \<or> i = 4 \<or> i = 5 \<or> i =6" 
+by (auto)
+lemma in6 : "i \<in> 6 \<Longrightarrow> i = 0 \<or> i = 1 \<or> i = 2 \<or> i = 3 \<or> i = 4 \<or> i = 5" 
+by (auto)
+lemma tonto : "xf \<in> nat \<Longrightarrow> x \<in> nat \<Longrightarrow> succ(succ(succ(succ(succ(succ(xf)))))) \<in> succ(succ(succ(succ(succ(succ(succ(x))))))) \<Longrightarrow> xf \<le> x"
+  by(rule ltI,rule ltD,auto,rule lt_trans[of _ "succ(succ(succ(succ(succ(succ(xf))))))"],simp,rule leI,rule ltI,assumption,simp)
+  
+lemma perm_sep_env: "{p,q,r,s,t,u,w} \<subseteq> M \<Longrightarrow> env \<in> list(M) \<Longrightarrow>
+  perm_list(fUg(length(env)),[t,s,w,p,q,r,u]@env) = [p,q,r,s,t,u]@env@[w]"
+  apply(rule nth_equalityI)
+  apply(rule perm_list_tc[of _ "M"],simp,(subst env_len2,assumption+)+)
+  apply(rule fUg_bij,simp,simp add:app_type)
+  apply(subst perm_list_length[of _ "M"],simp,(subst env_len2,assumption+)+)
+  apply(rule fUg_bij,simp,simp)
+  apply(subst (asm) perm_list_length[of _ "M"],simp,(subst env_len2,assumption+)+)
+  apply(rule fUg_bij,simp)
+   apply(subst (asm) env_len2,assumption+)
+   apply(subst nth_perm[of _ "M"],simp)
+  apply(subst env_len2,assumption+)+
+  apply(rule fUg_bij,simp,subst env_len2,assumption+,erule ltD,drule ltD)
+  apply(subst (asm) ble3,simp,rule_tac c="i" in UnE,assumption)
+  apply(unfold fUg_def)
+   apply(subst fun_disjoint_apply1,subst dom_f)
+    prefer 3
+    apply(subst fun_disjoint_apply2,subst domain_of_fun,rule g_tc)
+     prefer 2
+    apply(rule_tac c="i" and A="6" in UnE,assumption) 
+    apply(drule in6)
+    apply(rule disjE,assumption,subst apply_fun,rule f_tc,simp,simp add:f_def,simp)
+    apply(rule_tac P="i=1" in disjE,assumption,subst apply_fun,rule f_tc,simp,simp add:f_def,simp)
+   apply(rule_tac P="i=2" in disjE,assumption,subst apply_fun,rule f_tc,simp,simp add:f_def,simp add:nth_append)
+    apply(rule_tac P="i=3" in disjE,assumption,subst apply_fun,rule f_tc,simp,simp add:f_def,simp)
+    apply(rule_tac P="i=4" in disjE,assumption,subst apply_fun,rule f_tc,simp,simp add:f_def,simp)
+    apply(subst apply_fun,rule f_tc,simp,simp add:f_def,simp)
+   apply(subst apply_fun,rule f_tc,simp,simp add:f_def,simp,simp add:nth_append,clarsimp)
+    apply(rule ble7,rule ble5,simp,rule ble6,rule ble5,simp)
+  apply(unfold g_def,subst beta,assumption)
+  apply(simp)
+  apply(rule_tac n="length(env)" in natE,simp+)
+  apply(rule_tac n="i" in natE,simp+,subgoal_tac "i\<in>6",clarsimp,rule ltD,simp)  
+  apply(rule_tac n="xa" in natE,simp+,subgoal_tac "xa\<in>6",clarsimp,rule ltD,simp)
+  apply(rule_tac n="xb" in natE,simp+,subgoal_tac "xa\<in>6",clarsimp,rule ltD,simp+)
+  apply(rule_tac n="xc" in natE,simp+,subgoal_tac "xa\<in>6",clarsimp,rule ltD,simp+)
+  apply(rule_tac n="xd" in natE,simp+,subgoal_tac "xa\<in>6",clarsimp,rule ltD,simp+)
+  apply(rule_tac n="xe" in natE,simp+,clarsimp)
+  apply(subst (asm) nth_append,simp+,drule_tac xf="xf" and x="x" in tonto,simp+)
+done
+
+lemma perm_sep_env2: "{p,q,r,s,t,u,w} \<subseteq> M \<Longrightarrow> env \<in> list(M) \<Longrightarrow>
+  perm_list(converse(fUg(length(env))),[p,q,r,s,t,u]@env@[w]) = [t,s,w,p,q,r,u]@env"
+ apply(rule nth_equalityI)
+  apply(rule perm_list_tc[of _ "M"],simp,simp add:app_type,(subst env_len,assumption+)+)
+  apply(rule fUg_conv_bij,simp,simp add:app_type)
+  apply(subst perm_list_length[of _ "M"],simp add:app_type,(subst env_len,assumption+)+)
+  apply(rule fUg_conv_bij,simp,simp)
+  apply(subst (asm) perm_list_length[of _ "M"],simp add:app_type,(subst env_len,assumption+)+)
+  apply(rule fUg_conv_bij,simp)
+   apply(subst (asm) env_len,assumption+)
+   apply(subst nth_perm[of _ "M"],simp add:app_type)
+  apply(subst env_len,assumption+)+
+  apply(rule fUg_conv_bij,simp,subst env_len,assumption+,erule ltD,drule ltD)
+  apply(subst perm_sep_env[symmetric],assumption+)
+  apply(subst nth_perm_conv[of _ "M"],simp add:app_type,(subst env_len2,assumption+)+)
+  apply(rule fUg_bij,simp,(subst env_len2,assumption+)+,simp)
+done
+  
 context forcing_thms begin  
 
 lemmas transitivity = Transset_intf trans_M
@@ -61,9 +332,9 @@ notepad begin   (************** notepad **************)
     assume
       "params\<in>list(M)"
     let 
-      ?lenenv="length(params)#+7"    
+      ?lenenv="length(params)"    
     let
-      ?new_form="rename(forces(?\<chi>))`?lenenv`converse(perm_sep_forces(?lenenv))"
+      ?new_form="rename(forces(?\<chi>))`(7#+?lenenv)`fUg(?lenenv)"
     let
       ?\<psi>="Exists(Exists(And(pair_fm(0,1,2),?new_form)))"
     from \<open>params\<in>list(M)\<close> have
@@ -72,11 +343,12 @@ notepad begin   (************** notepad **************)
       "arity(?\<chi>) \<le> length(params)#+3" 
       by (simp add:nat_union_abs1, simp add:nat_union_abs2)
     with phi have
-      "arity(forces(?\<chi>)) \<le> ?lenenv"
+      "arity(forces(?\<chi>)) \<le> ?lenenv#+7"
       using arity_forces by simp
-    with phi conv_perm_sep_bij arity_forces \<open>?lenenv \<in> nat\<close> have
-      "?new_form \<in> formula"
-      using ren_tc by simp
+    with phi definability[of "?\<chi>"] fUg_bij[of ?lenenv] arity_forces \<open>?lenenv \<in> nat\<close> have
+      nf_form : "?new_form \<in> formula"
+      using ren_lib_tc[of "forces(?\<chi>)" _ "fUg(?lenenv)"]  \<open>?lenenv \<in> nat\<close>
+        by(simp)
     then have
       "?\<psi> \<in> formula"
       by simp
@@ -103,7 +375,7 @@ notepad begin   (************** notepad **************)
         then have
           "[\<theta>,\<pi>]@params@[u] \<in> list(M)" by simp
         let
-          ?new_env="perm_list(perm_sep_forces(?lenenv),?Pl1@[p,\<theta>,\<pi>]@params@[u])"
+          ?new_env="perm_list(converse(fUg(?lenenv)),?Pl1@[p,\<theta>,\<pi>]@params@[u])"
         let
           ?\<psi>="Exists(Exists(And(pair_fm(0,1,2),?new_form)))"
         have
@@ -118,24 +390,26 @@ notepad begin   (************** notepad **************)
         from in_M have
           "?Pl1 \<in> list(M)" by simp
         from in_M have
-          len : "?lenenv = length(?Pl1@[p,\<theta>,\<pi>]@params@[u])" 
-          using \<open>?lenenv\<in>nat\<close> length_app by simp 
+          len : "7#+?lenenv = length(?Pl1@[p,\<theta>,\<pi>]@params@[u])" 
+          using \<open>?lenenv\<in>nat\<close>  by simp 
         have
-          Eq1': "?new_env = [\<theta>,p,u]@?Pl1@[\<pi>]@params"
-          using perm_sep_env  by simp
+          Eq1': "?new_env = [\<theta>,p,u,P,leq,one,\<pi>]@params"
+          using in_M perm_sep_env2 app_type
+            by simp
         then have
           "sats(M,?new_form,[\<theta>,p,u]@?Pl1@[\<pi>]@params) \<longleftrightarrow> sats(M,?new_form,?new_env)"
           by simp
         also have
           "sats(M,?new_form,?new_env) \<longleftrightarrow> 
-        sats(M,rename(forces(?\<chi>))`length(?Pl1@[p,\<theta>,\<pi>]@params@[u])`converse(perm_sep_forces(length(params)#+7)),?new_env)" 
-          using len
+           sats(M,rename(forces(?\<chi>))`(7#+length(params))`fUg(length(params)),?new_env)"           
           by simp
-        also have
+        have
           "... \<longleftrightarrow> sats(M,forces(?\<chi>),?Pl1@[p,\<theta>,\<pi>]@params@[u])"
           using  phi in_M  transD trans_M arit_fact
-          apply(rule_tac ren_Sat_leq [symmetric])
-             apply(auto simp add: perm_sep_bij arity_forces nat_union_abs1)
+          apply(subst conv_fUgInv_eq,simp,subst conv_fUg_eq,simp)
+          apply(subst len,rule ren_Sat_leq[symmetric],simp,simp add:app_type)
+          apply(subst (1 2) len[symmetric],rule fUgInv_bij)
+           apply(auto simp add: arity_forces nat_union_abs1)
           done
         also have
           "... \<longleftrightarrow> sats(M,forces(?\<chi>), [P, leq, one,p,\<theta>,\<pi>]@(params@[u]))" by simp
@@ -357,7 +631,7 @@ notepad begin   (************** notepad **************)
      \<pi> \<in> M \<Longrightarrow> \<sigma> \<in> M \<Longrightarrow> domain(\<pi>) \<times> P \<in> M \<Longrightarrow>  domain(\<pi>) \<in> M \<Longrightarrow>
      {u \<in> domain(\<pi>) \<times> P .
         sats(M, Exists(Exists(And(pair_fm(0, 1, 2), rename(forces(And(Member(0, 1), \<phi>))) ` 
-          (length(params)#+7) ` converse(perm_sep_forces(length(params)#+7))))),
+          (7#+length(params)) ` fUg(length(params))))),
          [u] @ [P, leq, one] @ [\<pi>] @ params)} \<in>  M \<Longrightarrow>
      {u \<in> domain(\<pi>) \<times> P .
        \<exists>\<theta>\<in>M. \<exists>p\<in>P. u = \<langle>\<theta>, p\<rangle> \<and> (p \<in> G \<longrightarrow> val(G, \<theta>) \<in> val(G, \<pi>) \<and> sats(M[G], \<phi>, [val(G, \<theta>), val(G, \<pi>)]))} \<in> M 
@@ -370,7 +644,7 @@ notepad begin   (************** notepad **************)
      \<pi> \<in> M" "\<sigma> \<in> M" "domain(\<pi>) \<times> P \<in> M" " domain(\<pi>) \<in> M" "
      {u \<in> domain(\<pi>) \<times> P .
         sats(M, Exists(Exists(And(pair_fm(0, 1, 2), rename(forces(And(Member(0, 1), \<phi>))) ` 
-          (length(params)#+7) ` converse(perm_sep_forces(length(params)#+7))))),
+          (7#+length(params)) ` fUg(length(params))))),
          [u] @ [P, leq, one] @ [\<pi>] @ params)} \<in>  M" "
      {u \<in> domain(\<pi>) \<times> P .
        \<exists>\<theta>\<in>M. \<exists>p\<in>P. u = \<langle>\<theta>, p\<rangle> \<and> (p \<in> G \<longrightarrow> val(G, \<theta>) \<in> val(G, \<pi>) \<and> sats(M[G], \<phi>, [val(G, \<theta>), val(G, \<pi>)]))} \<in> M"
